proof/amd64/avx2/Keccak1600_avx2.ec
@@ -1,0 +1,114 @@
+(******************************************************************************
+   Keccak1600_avx2.ec:
+
+   Correctness proof for the Keccak AVX2 implementation
+
+
+
+******************************************************************************)
+
+require import List Real Distr Int IntDiv CoreMap.
+
+from Jasmin require import JModel.
+
+from CryptoSpecs require export Keccakf1600_Spec.
+
+require import WArray768.
+from JazzEC require import Jazz_avx2.
+
+require import Array4 Array5 Array7 Array24 Array25.
+
+from CryptoSpecs require import FIPS202_Keccakf1600.
+from CryptoSpecs require import Keccakf1600_Spec.
+
+(* circuit-friendly state mappings *)
+
+abbrev u256_bits64 (w: W256.t) k : W64.t =
+ W64.init (fun i => w.[i+64*k]).
+
+lemma u256_bits64E w k:
+ 0 <= k < 4 =>
+ u256_bits64 w k = w \bits64 k.
+proof.
+move=> Hk; rewrite /u256_bits64.
+apply W64.ext_eq => i Hi.
+by rewrite bits64E initiE 1://= initiE 1://= /#.
+qed.
+
+op u256_pack4 (w0 w1 w2 w3: W64.t): W256.t =
+ W256.init (fun i => if i < 64 then w0.[i]
+                     else if i < 128 then w1.[i-64]
+                     else if i < 192 then w2.[i-128]
+                     else w3.[i-192]).
+
+
+lemma u256_pack4E w0 w1 w2 w3:
+ u256_pack4 w0 w1 w2 w3 = pack4 [w0; w1; w2; w3].
+proof.
+rewrite /u256_pack4; apply W256.ext_eq => k Hk.
+rewrite initiE 1:// pack4E initiE 1:// /=.
+rewrite get_of_list 1:/# /=.
+case: (k < 64) => C1.
+ by rewrite ifT 1:/# modz_small /= /#.
+case: (k < 128) => C2.
+ by rewrite ifF 1:/# ifT 1:/#; congr; smt().
+case: (k < 192) => C3.
+ by rewrite ifF 1:/# ifF 1:/# ifT 1:/#; congr; smt().
+by rewrite ifF 1:/# ifF 1:/# ifF 1:/# ifT 1:/#; congr => /#.
+qed.
+
+op stavx2_from_st25 (st: W64.t Array25.t): W256.t Array7.t =
+ Array7.of_list W256.zero
+  [ u256_pack4 st.[ 0] st.[ 0] st.[ 0] st.[ 0]
+  ; u256_pack4 st.[ 1] st.[ 2] st.[ 3] st.[ 4]
+  ; u256_pack4 st.[10] st.[20] st.[ 5] st.[15]
+  ; u256_pack4 st.[16] st.[ 7] st.[23] st.[14]
+  ; u256_pack4 st.[11] st.[22] st.[ 8] st.[19]
+  ; u256_pack4 st.[21] st.[17] st.[13] st.[ 9]
+  ; u256_pack4 st.[ 6] st.[12] st.[18] st.[24]
+  ].
+
+op stavx2_to_st25 (st: W256.t Array7.t): W64.t Array25.t =
+ Array25.of_list W64.zero
+  [ u256_bits64 st.[0] 0; u256_bits64 st.[1] 0; u256_bits64 st.[1] 1; u256_bits64 st.[1] 2; u256_bits64 st.[1] 3
+  ; u256_bits64 st.[2] 2; u256_bits64 st.[6] 0; u256_bits64 st.[3] 1; u256_bits64 st.[4] 2; u256_bits64 st.[5] 3
+  ; u256_bits64 st.[2] 0; u256_bits64 st.[4] 0; u256_bits64 st.[6] 1; u256_bits64 st.[5] 2; u256_bits64 st.[3] 3
+  ; u256_bits64 st.[2] 3; u256_bits64 st.[3] 0; u256_bits64 st.[5] 1; u256_bits64 st.[6] 2; u256_bits64 st.[4] 3
+  ; u256_bits64 st.[2] 1; u256_bits64 st.[5] 0; u256_bits64 st.[4] 1; u256_bits64 st.[3] 2; u256_bits64 st.[6] 3
+  ].
+
+lemma stavx2_from_st25K st:
+ stavx2_to_st25 (stavx2_from_st25 st) = st.
+proof.
+rewrite /stavx2_to_st25 /stavx2_from_st25 !u256_bits64E 1..25:// /=.
+rewrite !u256_pack4E /=.
+by apply Array25.all_eq_eq; rewrite /all_eq.
+qed.
+
+op u256_broadcastP w =
+ u256_bits64 w 1 = u256_bits64 w 0
+ /\ u256_bits64 w 2 = u256_bits64 w 0
+ /\ u256_bits64 w 3 = u256_bits64 w 0.
+
+lemma u256_broadcastP_VPBROADCAST w:
+ u256_broadcastP (VPBROADCAST_4u64 w).
+proof.
+rewrite /VPBROADCAST_4u64 /u256_broadcastP.
+by rewrite !u256_bits64E 1..4:// !pack4bE 1..4:// /= -iotaredE /=.
+qed.
+
+lemma u256_broadcastP_xor w1 w2:
+ u256_broadcastP w1 =>
+ u256_broadcastP w2 =>
+ u256_broadcastP (w1 `^` w2).
+proof.
+by rewrite /u256_broadcastP !u256_bits64E 1..12:// !xorb64E /#.
+qed.
+
+
+abbrev stF_avx2 f = fun st => stavx2_from_st25 (f (stavx2_to_st25 st)).
+
+op stavx2_keccakf1600 = stF_avx2 keccak_f1600_op.
+
+
+
