proof/amd64/avx2/Keccak1600_avx2x4.ec
@@ -1,0 +1,188 @@
+(******************************************************************************
+   Keccak1600_avx2x4.ec:
+
+   Correctness proof for the 4x_AVX2 implementation
+
+
+
+******************************************************************************)
+
+require import List Real Distr Int IntDiv CoreMap.
+
+from Jasmin require import JModel.
+
+from CryptoSpecs require import FIPS202_SHA3 FIPS202_Keccakf1600.
+from CryptoSpecs require import Keccakf1600_Spec.
+
+require import WArray768.
+from JazzEC require import Jazz_avx2.
+from JazzEC require import Array24 Array5.
+
+
+
+
+(** lemmata (move?) *)
+
+
+import Ring.IntID.
+
+lemma bits8_bits (w: W256.t) (k: int):
+ w \bits8 k = W8.bits2w (bits w (8*k) 8).
+proof.
+by rewrite -all_eqP /all_eq /bits /mkseq -iotaredE /= /#.
+qed.
+
+lemma bits64_bits (w: W256.t) (k: int):
+ w \bits64 k = W64.bits2w (bits w (64*k) 64).
+proof.
+by rewrite -all_eqP /all_eq /bits /mkseq -iotaredE /= /#.
+qed.
+
+(* useful to eval constants... *)
+lemma bits8_red (w: W256.t) (k: int):
+ 0 <= k =>
+ w \bits8 k
+ = W8.of_int (to_uint w %/ (2^(8*k)) %% 2^8).
+proof.
+move=> Hk; rewrite bits8_bits.
+apply W8.word_modeqP.
+rewrite of_uintK !modz_mod.
+rewrite W8.to_uintE bits2wK 1:size_bits //.
+by rewrite bits_divmod 1..2:/# modz_mod.
+qed.
+
+lemma bits64_red (w: W256.t) (k: int):
+ 0 <= k =>
+ w \bits64 k
+ = W64.of_int (to_uint w %/ (2^(64*k)) %% 2^64).
+proof.
+move=> Hk; rewrite bits64_bits.
+apply W64.word_modeqP.
+rewrite of_uintK !modz_mod.
+rewrite W64.to_uintE bits2wK 1:size_bits //.
+by rewrite bits_divmod 1..2:/# modz_mod.
+qed.
+
+lemma get256_init256 (a: W256.t Array24.t) i:
+ 0 <= i < 24 =>
+ get256 (init256 ("_.[_]" a)) i = a.[i].
+proof.
+move=> Hi; rewrite /get256_direct /init256 -(unpack8K a.[i]).
+congr; apply W32u8.Pack.ext_eq => x Hx.
+rewrite initiE //= unpack8E !initiE 1..2:/# /=; congr.
+ congr; smt().
+smt().
+qed.
+
+
+
+(** Packed 4x-state *)
+type state4x = W256.t Array25.t.
+
+op (\a25bits64) (a: state4x) (k: int): state =
+ Array25.map (fun (x: W256.t) => W4u64.\bits64 x k) a.
+
+op (\a24bits64) (a: W256.t Array24.t) (k: int): W64.t Array24.t =
+ Array24.map (fun (x: W256.t) => W4u64.\bits64 x k) a.
+
+op (\a5bits64) (a: W256.t Array5.t) (k: int): W64.t Array5.t =
+ Array5.map (fun (x: W256.t) => W4u64.\bits64 x k) a.
+
+op a25pack4 (l: state list): state4x =
+ Array25.init (fun i => pack4 (map (fun (s: state) => s.[i]) l)).
+
+op a25unpack4 (st4: state4x): state list =
+ map (fun k=> st4 \a25bits64 k) (iota_ 0 4).
+
+lemma a25bits64iE x k i:
+ 0 <= i < 25 =>
+ (x \a25bits64 k).[i] = x.[i] \bits64 k.
+proof. by move=> Hi; rewrite mapiE //. qed.
+
+lemma a24bits64iE x k i:
+ 0 <= i < 24 =>
+ (x \a24bits64 k).[i] = x.[i] \bits64 k.
+proof. by move=> Hi; rewrite mapiE //. qed.
+
+lemma a5bits64iE x k i:
+ 0 <= i < 5 =>
+ (x \a5bits64 k).[i] = x.[i] \bits64 k.
+proof. by move=> Hi; rewrite mapiE //. qed.
+
+lemma a25unpack4K s4:
+ a25pack4 (a25unpack4 s4) = s4.
+proof.
+rewrite /a25pack4 /a25unpack4.
+apply Array25.ext_eq => i Hi; rewrite initiE //=.
+rewrite -iotaredE /= !a25bits64iE //=.
+rewrite -{5}(unpack64K s4.[i]); congr.
+by rewrite unpack64E init_of_list -iotaredE /=. 
+qed.
+
+lemma a25pack4_bits64 k (stl: state list):
+ 0 <= k < 4 =>
+ a25pack4 stl \a25bits64 k = nth st0 stl k.
+proof.
+move=> Hk; apply Array25.ext_eq => i Hi.
+rewrite mapiE //= initiE //= pack4bE //=.
+rewrite of_listE initiE //=.
+case: (k < size stl) => E.
+ by rewrite (nth_map st0) 1:/#.
+rewrite !nth_out; first 2 by smt(size_map).
+by rewrite createiE.
+qed.
+
+op a5pack4 (l: (W64.t Array5.t) list): W256.t Array5.t =
+ Array5.init (fun i => pack4 (map (fun (x: W64.t Array5.t) => x.[i]) l)).
+
+op match_state4x (st0 st1 st2 st3: state) (st4x: state4x) =
+ st4x = a25pack4 [st0; st1; st2; st3].
+
+lemma a25pack4_eq stl st4x:
+ a25pack4 stl = st4x
+ <=>
+ all (fun k=>st4x \a25bits64 k = nth st0 stl k) (iota_ 0 4).
+proof.
+split.
+ move => <-; apply/List.allP => k. 
+ rewrite mem_iota => Hk /=; apply a25pack4_bits64; smt().
+move=> /List.allP H.
+apply Array25.ext_eq => i Hi.
+rewrite initiE //=.
+rewrite -(unpack64K st4x.[i]); congr.
+apply W4u64.Pack.ext_eq => k Hk.
+rewrite of_listE unpack64E !initiE //=.
+rewrite -a25bits64iE // H; first smt(mem_iota).
+case: (k < size stl) => E.
+ by rewrite (nth_map st0) 1:/#.
+rewrite !nth_out; first 2 by smt(size_map).
+by rewrite createiE.
+qed.
+
+lemma a5bits64_set (c: W256.t Array5.t) x y i:
+ 0 <= i < 4 =>
+ 0 <= x < 5 =>
+ c.[x <- y] \a5bits64 i
+ = (c \a5bits64 i).[x <- y \bits64 i].
+proof.
+move=> Hi Hx; apply Array5.ext_eq => j Hj.
+rewrite a5bits64iE 1:// !get_setE 1..2:/#.
+case: (j=x) => E //.
+by rewrite a5bits64iE.
+qed.
+
+lemma xorw_bits64 (w1 w2: W256.t) k:
+ 0 <= k < 4 =>
+ w1 `^` w2 \bits64 k = (w1 \bits64 k) `^` (w2 \bits64 k).
+proof.
+move=> Hk; rewrite -{1}(unpack64K w1) -{1}(unpack64K w2). 
+by rewrite xorb4u64E pack4bE // map2iE // !unpack64E !initiE.
+qed.
+
+
+
+
+(******************)
+
+
+
